rt ainvs: proof update for domain_time fix
Signed-off-by: Michael McInerney <m.mcinerney@unsw.edu.au>

proof/invariant-abstract/Syscall_AI.thy
@@ -1563,6 +1563,138 @@ lemma handle_invocation_not_blocking_not_calling_first_phase_ct_active[wp]:
               elim: st_tcb_ex_cap)
   done
 
+lemma asdfkjhksjhdf[wp]:
+   "\<lbrace>\<lambda>s. \<not>is_cur_domain_expired s \<longrightarrow> scheduler_action s = resume_cur_thread\<rbrace>
+    check_budget_restart
+    \<lbrace>\<lambda>rv s. rv \<longrightarrow> scheduler_action s = resume_cur_thread\<rbrace>"
+   unfolding check_budget_restart_def check_budget_def
+   by (wpsimp wp: gts_wp)
+
+definition reprogram_timer_independent_A :: "('z state \<Rightarrow> bool) \<Rightarrow> bool" where
+   "reprogram_timer_independent_A P \<equiv> \<forall>f s. P s \<longrightarrow> P (s\<lparr>reprogram_timer := f (reprogram_timer s)\<rparr>)"
+
+ lemma reprogram_timer_independent_AI[intro!, simp]:
+   "\<lbrakk>\<And>s f. P (s\<lparr>reprogram_timer := f (reprogram_timer s)\<rparr>) = P s\<rbrakk>
+    \<Longrightarrow> reprogram_timer_independent_A P"
+   by (simp add: reprogram_timer_independent_A_def)
+
+ lemma reprogram_timer_independent_A_conjI[intro!]:
+   "\<lbrakk>reprogram_timer_independent_A P; reprogram_timer_independent_A Q\<rbrakk>
+    \<Longrightarrow> reprogram_timer_independent_A (P and Q)"
+   "\<lbrakk>reprogram_timer_independent_A P; reprogram_timer_independent_A Q\<rbrakk>
+    \<Longrightarrow> reprogram_timer_independent_A (\<lambda>s. P s \<and> Q s)"
+   by (auto simp: reprogram_timer_independent_A_def)
+
+
+lemma is_cur_domain_expired_lift:
+   assumes x: "\<And>P. f \<lbrace>\<lambda>s. P (domain_time s)\<rbrace>"
+   shows "f \<lbrace>is_cur_domain_expired\<rbrace>"
+   unfolding is_cur_domain_expired_def
+   by (wp x)
+
+lemma check_domain_time_inv:
+   shows "\<lbrakk>
+           reprogram_timer_independent_A P\<rbrakk>
+          \<Longrightarrow> \<lbrace>P\<rbrace> check_domain_time \<lbrace>\<lambda>_ s. (\<not> is_cur_domain_expired s) \<longrightarrow> P s\<rbrace>"
+  apply (clarsimp simp: check_domain_time_def)
+  apply (rule hoare_seq_ext[OF _ gets_sp])
+  apply (rule hoare_when_cases)
+  apply clarsimp
+  apply (rule hoare_seq_ext_skip, wpsimp)
+apply (fastforce simp: reprogram_timer_independent_A_def is_cur_domain_expired_def)
+    apply (wpsimp wp: hoare_vcg_imp_lift' is_cur_domain_expired_lift)
+    apply (rule hoare_pre_cont)
+   apply (wpsimp simp: is_cur_domain_expired_def hoare_vcg_if_lift2 wp: gets_wp)
+   done
+
+lemma update_time_stamp_inv:
+   shows "\<lbrakk>time_state_independent_A P;
+          domain_time_independent_A P;  getCurrentTime_independent_A P;
+update_time_stamp_independent_A P;
+          cur_time_independent_A P\<rbrakk>
+          \<Longrightarrow> \<lbrace>P\<rbrace> update_time_stamp \<lbrace>\<lambda>_ s. (\<not> is_cur_domain_expired s) \<longrightarrow> P s\<rbrace>"
+  apply (clarsimp simp: update_time_stamp_def commit_domain_time_def num_domains_def)
+   apply (rule hoare_seq_ext_skip, wpsimp)
+   apply (rule hoare_seq_ext_skip, wpsimp)
+   apply (rule hoare_seq_ext_skip, wpsimp)
+    apply (fastforce simp: cur_time_independent_A_def)
+   apply (rule hoare_seq_ext_skip, wpsimp)+
+
+    apply (fastforce simp:  update_time_stamp_independent_A_def)
+   apply (rule hoare_seq_ext_skip, wpsimp)+
+apply wpsimp
+    apply (fastforce simp: domain_time_independent_A_def)
+done
+
+crunches check_domain_time
+  for invs[wp]: invs
+  and ct_active[wp]: ct_active
+  and asdf[wp]: "\<lambda>s. st_tcb_at active (cur_thread s) s"
+  and asdf2[wp]: "\<lambda>s. ex_nonz_cap_to (cur_thread s) s"
+  (simp: crunch_simps wp: crunch_wps)
+
+lemma bind_liftE_distrib': "(liftE (A >>= (\<lambda>x. B))) = (liftE A >>=E (\<lambda>x. liftE (\<lambda>s. B s)))"
+  apply (clarsimp simp: liftE_def bindE_def lift_def bind_assoc)
+  done
+
+lemma set_scheduler_action_is_schedulable_bool_cur_thread[wp]:
+  "set_scheduler_action sa \<lbrace>\<lambda>s. is_schedulable_bool (cur_thread s) s\<rbrace>"
+  apply (clarsimp simp: set_scheduler_action_def)
+  apply (wpsimp wp: modify_wp)
+  apply (clarsimp simp: is_schedulable_bool_def' get_tcb_def opt_map_red in_release_queue_def)
+  done
+
+lemma set_tcb_queue_wp:
+  "\<lbrace>\<lambda>s. P (ready_queues_update (\<lambda>qs d p. if d = t \<and> p = prio then queue else qs d p) s)\<rbrace>
+   set_tcb_queue t prio queue
+   \<lbrace>\<lambda>_. P\<rbrace>"
+  by (wpsimp simp: set_tcb_queue_def) (auto elim!: rsubst[of P])
+
+lemma tcb_sched_action_schedulable_bool[wp]:
+  "\<lbrace>\<lambda>s. is_schedulable_bool t s\<rbrace>
+   tcb_sched_action f t
+   \<lbrace>\<lambda>rv s. is_schedulable_bool t s\<rbrace>"
+  apply (wpsimp simp: tcb_sched_action_def thread_set_def thread_get_def get_tcb_queue_def
+                  wp: set_object_wp set_tcb_queue_wp)
+  by (fastforce simp: is_schedulable_bool_def' get_tcb_rev obj_at_def dest!: get_tcb_SomeD split: option.splits)
+
+lemma tcb_sched_action_schedulable_bool_cur_thread[wp]:
+  "\<lbrace>\<lambda>s. is_schedulable_bool (cur_thread s) s\<rbrace>
+   tcb_sched_action f t
+   \<lbrace>\<lambda>rv s. is_schedulable_bool (cur_thread s) s\<rbrace>"
+  apply (wpsimp simp: tcb_sched_action_def thread_set_def thread_get_def get_tcb_queue_def
+                  wp: set_object_wp set_tcb_queue_wp)
+  by (fastforce simp: is_schedulable_bool_def' get_tcb_rev obj_at_def dest!: get_tcb_SomeD split: option.splits)
+
+lemma reschedule_required_is_schedulable_bool[wp]:
+  "reschedule_required \<lbrace>\<lambda>s. is_schedulable_bool (cur_thread s) s\<rbrace>"
+  apply (clarsimp simp: reschedule_required_def)
+  apply (rule hoare_seq_ext[OF _ gets_sp])
+  apply (rule hoare_seq_ext)
+   apply wpsimp
+  apply (case_tac action; clarsimp)
+    apply wpsimp
+prefer 2
+apply wpsimp
+  apply (rule hoare_seq_ext[OF _ is_schedulable_sp'])
+  apply (rule hoare_when_cases, simp)
+apply (wpsimp wp: thread_get_wp)+
+  apply (clarsimp simp: is_schedulable_bool_def' tcb_at_def get_tcb_def pred_tcb_at_def obj_at_def is_tcb_def)
+done
+
+lemma check_domain_time_is_schedulable_bool[wp]:
+  "check_domain_time \<lbrace>\<lambda>s. is_schedulable_bool (cur_thread s) s\<rbrace>"
+  apply (clarsimp simp: check_domain_time_def)
+  apply (rule hoare_seq_ext[OF _ gets_sp])
+  apply (rule hoare_when_cases)
+  apply clarsimp
+  apply (rule hoare_seq_ext_skip, wpsimp)
+  apply (clarsimp simp: is_schedulable_bool_def' tcb_at_def get_tcb_def pred_tcb_at_def obj_at_def is_tcb_def
+in_release_queue_def is_cur_domain_expired_def)
+apply wpsimp
+   done
+
+
 lemma he_invs[wp]:
   "\<And>e.
     \<lbrace>\<lambda>s. invs s \<and> (e \<noteq> Interrupt \<longrightarrow> ct_running s) \<and>
@@ -1573,12 +1705,15 @@ lemma he_invs[wp]:
   apply (case_tac e, simp_all)
        apply (rename_tac syscall)
        apply (case_tac syscall, simp_all)
-                 by (wpsimp wp: hoare_vcg_imp_conj_lift' check_budget_restart_true
-                          comb: hoare_drop_imps hoare_drop_imp_conj'
-                          simp: if_apply_def2 valid_fault_def
-                     | wps | erule active_from_running
-                     | fastforce simp: tcb_at_invs ct_in_state_def valid_fault_def
-                                elim!: st_tcb_ex_cap dest: active_from_running)+
+              apply (wpsimp wp: hoare_vcg_imp_conj_lift' check_domain_time_inv update_time_stamp_inv
+                           comb: hoare_drop_imps hoare_drop_imp_conj'
+                           simp: if_apply_def2 valid_fault_def
+                      | wpsimp wp: check_budget_restart_true
+                      | wps | erule active_from_running
+                      | fastforce simp: tcb_at_invs ct_in_state_def valid_fault_def
+                                 elim!: st_tcb_ex_cap dest: active_from_running
+| clarsimp simp: ct_in_state_def pred_tcb_at_def obj_at_def)+
+  done
 
 end
 
