proof/invariant-abstract/Deterministic_AI.thy
@@ -3975,6 +3975,7 @@ global_interpretation reset_work_units_ext_extended: is_extended "reset_work_uni
 
 lemma preemption_point_inv':
   "\<lbrakk>irq_state_independent_A P; time_state_independent_A P; getCurrentTime_independent_A P;
+domain_time_independent_A P;
     update_time_stamp_independent_A P; cur_time_independent_A P;
     \<And>f s. P (work_units_completed_update f s) = P s\<rbrakk>
    \<Longrightarrow> \<lbrace>P\<rbrace> preemption_point \<lbrace>\<lambda>_. P\<rbrace>"
@@ -3986,6 +3987,7 @@ lemma preemption_point_inv':
   apply (rule alternative_valid; (solves wpsimp)?)
   apply (rule validE_valid)
   apply (rule hoare_seq_ext_skipE, (solves \<open>wpsimp simp: reset_work_units_def\<close>)?)+
+apply (wpsimp wp: update_time_stamp_wp)
   apply (wpsimp wp: hoare_vcg_all_lift hoare_drop_imps update_time_stamp_wp)
   done
 
@@ -4168,7 +4170,8 @@ crunches cap_delete_one, restart
 
 context notes if_cong[cong] begin
 
-crunch valid_list[wp]: update_time_stamp "valid_list"
+crunches update_time_stamp, check_domain_time
+  for valid_list[wp]: valid_list
   (wp: get_object_wp)
 
 crunch valid_list[wp]: reply_from_kernel "valid_list"
